SEIO*: spec contexts as pre-conditions in RQ

seiostar/QTypes.OpenValComp.fst
@@ -6,100 +6,56 @@ open IOStar
 include QTypes.TypEnv
 include QTypes.EvalEnv
 
-module M = FStar.Monotonic.Pure
-unfold
-let mk_pure_wp #a (wp:pure_wp' a{M.is_monotonic wp}) : pure_wp a =
-  M.intro_pure_wp_monotonicity wp; wp
-
 (** F* works better with these functions because it helps dealing with qTypes,
     even if they are synonyms *)
 
 type fs_val (t:qType) = get_Type t
 
-type spec_env (g:typ_env) (a:qType) =
-  eval_env g -> pure_wp (fs_val a)
+type spec_env (g:typ_env) =
+  eval_env g -> pure_pre
 
-type fs_oval (g:typ_env) (t:qType) (wpG:spec_env g t) =
-  fsG:eval_env g -> PURE (fs_val t) (wpG fsG)
+type fs_oval (g:typ_env) (t:qType) (pre:spec_env g) =
+  fsG:eval_env g -> Pure (fs_val t) (requires (pre fsG)) (ensures (fun _ -> True))
 
-let spec_env_return (#g:typ_env) (#a:qType) (x:fs_val a) : spec_env g a =
-  fun _ -> pure_return _ x
+let spec_env_return (#g:typ_env) (#a:qType) (x:fs_val a) : spec_env g =
+  fun _ -> True
 
 unfold
-val standard_spec_env_bind : #g:typ_env ->
-                    #a:qType ->
-                    #b:qType ->
-                    wpM : spec_env g a ->
-                    wpK : (spec_env (extend a g) b) ->
-                    spec_env g b
-let standard_spec_env_bind wpM wpK fsG =
-  M.elim_pure_wp_monotonicity (wpM fsG);
-  pure_bind_wp _ _ (wpM fsG) (fun x -> wpK (stack fsG x))
+let spec_env_bind (#g:typ_env) (#a:qType)
+  (preM:spec_env g) (preK:spec_env (extend a g)) : spec_env g =
+  fun fsG -> preM fsG /\ (forall (x:fs_val a). preK (stack fsG x))
 
-// let spec_env_bind' (#g:typ_env) (#a:qType) (#b:qType) (wpP:spec_env g a) (wpK:(fs_val a -> spec_env g b)) : spec_env g b =
-//   spec_env_bind wpP (fun fsG -> wpK (hd fsG) (tail fsG))
+let spec_env_bind' (#g:typ_env) (#a:qType)
+  (preP:spec_env g) (preK:(fs_val a -> spec_env g)) : spec_env g =
+  spec_env_bind preP (fun fsG -> preK (hd fsG) (tail fsG))
 
-(** [spec_env_bind] is a stronger bind for open computations (fs_ocomp).
-    Unlike [standard_spec_env_bind], the precondition requires the continuation's
-    precondition to hold for ALL values, not just the value returned by
-    the first computation. This is necessary because [io_bind] needs a
-    total continuation. *)
-unfold
-let spec_env_bind (#g:typ_env) (#a:qType) (#b:qType)
-  (wpM:spec_env g a) (wpK:spec_env (extend a g) b) : spec_env g b =
-  fun fsG ->
-    M.elim_pure_wp_monotonicity_forall ();
-    mk_pure_wp (fun p -> as_requires (wpM fsG) /\ (forall (x:fs_val a). wpK (stack fsG x) p))
+let spec_env_axiom (#g:typ_env) (#a:qType) : spec_env (extend a g) =
+  fun _ -> True
 
-let spec_env_bind' (#g:typ_env) (#a:qType) (#b:qType)
-  (wpP:spec_env g a) (wpK:(fs_val a -> spec_env g b)) : spec_env g b =
-  spec_env_bind wpP (fun fsG -> wpK (hd fsG) (tail fsG))
-
-let spec_env_axiom (#g:typ_env) (#a:qType) : spec_env (extend a g) a =
-  fun fsG -> pure_return _ (hd fsG)
-
-let spec_env_weaken (#g:typ_env) (#a #b:qType) (x:spec_env g a) : spec_env (extend b g) a =
+let spec_env_weaken (#g:typ_env) (#b:qType) (x:spec_env g) : spec_env (extend b g) =
   fun fsG -> x (tail fsG)
 
-let spec_env_index (#g:typ_env) (x:var{Some? (g x)}) : spec_env g (Some?.v (g x)) =
-  fun fsG -> pure_return _ (index fsG x)
+let spec_env_index (#g:typ_env) (x:var{Some? (g x)}) : spec_env g =
+  fun _ -> True
 
 val spec_env_app : #g :typ_env ->
-                #a :qType ->
-                #b :qType ->
-                wpF : spec_env g (a ^-> b) ->
-                wpX : spec_env g a ->
-                spec_env g b
-let spec_env_app #_ #a #b wpF wpX =
-  (fun fsG ->
-    pure_bind_wp _ _ (wpF fsG) (fun f' ->
-      pure_bind_wp _ _ (wpX fsG) (fun x' ->
-        pure_return _ (f' x'))))
-
-// let fs_ocomp_wp (g:typ_env) (t:qType) (wpG:spec_env g t) fsG : pure_wp (fs_comp t) =
-//   mk_pure_wp (fun (p:pure_post (fs_comp t)) ->
-//     forall (comp:fs_comp t). theta (comp) ⊑ wp_lift_pure_hist (wpG fsG) ==> p comp)
-  // CA: I think the previous would be intuitively what we want,
-  //     which could be simplified to the following since the operations
-  //     have no pre-conditions for now.
-  // Q:  The use of `as_requires` is weird, but we do not have a `p` to apply to `wpG`.
-  // mk_pure_wp (fun (p:pure_post (fs_comp t)) ->
-  //   as_requires (wpG fsG) /\ forall comp. p comp)
+                preF : spec_env g ->
+                preX : spec_env g ->
+                spec_env g
+let spec_env_app preF preX =
+  (fun fsG -> preF fsG /\ preX fsG)
 
 type fs_comp (t:qType) = io (fs_val t)
-// type fs_comp_ref (t:qType) (ref:fs_val t -> Type0) = io (r:(fs_val t){ref r})
 
-type fs_ocomp (g:typ_env) (t:qType) (wpG:spec_env g t) =
-  // fsG:eval_env g -> PURE (fs_comp t) (fs_ocomp_wp g t wpG fsG)
-  // fsG:eval_env g -> fs_comp_ref t (fun r -> wpG fsG `pure_stronger _` pure_return _ r)
-  fsG:eval_env g -> Pure (fs_comp t) (as_requires (wpG fsG)) (fun _ -> True)
+type fs_ocomp (g:typ_env) (t:qType) (pre:spec_env g) =
+  fsG:eval_env g -> Pure (fs_comp t) (requires (pre fsG)) (ensures (fun _ -> True))
 
-let spec_env_return_comp (#g:typ_env) (#a:qType) (comp:fs_comp a) : spec_env g a =
-  fun _ -> mk_pure_wp (fun (p:pure_post (fs_val a)) -> forall r. p r)
+let spec_env_return_comp (#g:typ_env) (#a:qType) (comp:fs_comp a) : spec_env g =
+  fun _ -> True
 
 
-let spec_env_return_oval (#g:typ_env) (#a:qType) #wpX (x:fs_oval g a wpX) : spec_env g a =
-  wpX
+let spec_env_return_oval (#g:typ_env) (#a:qType) #preX (x:fs_oval g a preX) : spec_env g =
+  preX
 
 (** Closed values **)
 let fs_val_if (#a:qType) (c:fs_val qBool) (e:fs_val a) (t:fs_val a) : fs_val a =
@@ -174,12 +130,11 @@ let fs_oval_fmap
   (#g:typ_env)
   (#a:qType)
   (#b:qType)
-  (#wpP : spec_env g a)
-  (m : fs_oval g a wpP)
+  (#preP : spec_env g)
+  (m : fs_oval g a preP)
   (f : fs_val a -> fs_val b)
-  : fs_oval g b (spec_env_bind' wpP (fun x -> spec_env_return (f x))) =
+  : fs_oval g b preP =
   fun fsG ->
-    M.elim_pure_wp_monotonicity (wpP fsG);
     f (m fsG)
 
 unfold
@@ -188,10 +143,9 @@ let fs_oval_axiom (g:typ_env) (t:qType)
   fun fsG -> hd fsG
 
 unfold
-let fs_oval_weaken (#g:typ_env) (#a:qType) (b:qType) (#wpX:spec_env g a) (x:fs_oval g a wpX)
-  : fs_oval (extend b g) a (spec_env_weaken wpX)
+let fs_oval_weaken (#g:typ_env) (#a:qType) (b:qType) (#preX:spec_env g) (x:fs_oval g a preX)
+  : fs_oval (extend b g) a (spec_env_weaken preX)
   = fun fsG ->
-    M.elim_pure_wp_monotonicity (wpX (tail fsG));
     x (tail fsG)
 
 unfold
@@ -203,14 +157,12 @@ unfold
 val fs_oval_app: #g : typ_env ->
                  #a : qType ->
                  #b : qType ->
-                 #wpF :spec_env g (a ^-> b) ->
-                 f :fs_oval g (a ^-> b) wpF ->
-                 #wpX : spec_env g a ->
-                 x :fs_oval g a wpX ->
-                 fs_oval g b (spec_env_app wpF wpX)
-let fs_oval_app #_ #_ #_ #wpF f #wpX x fsG =
-  M.elim_pure_wp_monotonicity (wpF fsG);
-  M.elim_pure_wp_monotonicity (wpX fsG);
+                 #preF :spec_env g ->
+                 f :fs_oval g (a ^-> b) preF ->
+                 #preX : spec_env g ->
+                 x :fs_oval g a preX ->
+                 fs_oval g b (spec_env_app preF preX)
+let fs_oval_app #_ #_ #_ #preF f #preX x fsG =
   (f fsG) (x fsG)
 
 
@@ -218,123 +170,99 @@ unfold
 val spec_env_lambda_tot : #g :typ_env ->
                 #a :qType ->
                 #b :qType ->
-                #wpBody:spec_env (extend a g) b ->
-                body:fs_oval (extend a g) b wpBody ->
-                spec_env g (a ^-> b)
+                #preBody:spec_env (extend a g) ->
+                body:fs_oval (extend a g) b preBody ->
+                spec_env g
 
-let spec_env_lambda_tot #g #a #b #wpBody body fsG : pure_wp (fs_val (a ^-> b)) by (
-  norm [delta_only [`%fs_val; `%op_Hat_Subtraction_Greater; `%get_Type]]
-)= (** Cezar: this looks exactly like what F* generates **)
-  mk_pure_wp (fun (p:pure_post (fs_val (a ^-> b))) ->
-    (forall (x:a._1). auto_squash (wpBody (stack fsG x) (fun _ -> True))) /\
-    (pure_bind_wp _ _
-      (pure_return (fs_val (a ^-> b)) (fun x -> body (stack fsG x))))
-      (pure_return (fs_val (a ^-> b))) p)
-    // pure_return (fs_val (a ^-> b)) (fun (x:a._1) -> body (stack fsG x)) p)
-    // p (fun (x:fs_val a) -> body (stack fsG x)))
+let spec_env_lambda_tot #g #a #b #preBody body fsG : pure_pre =
+  forall (x:fs_val a). preBody (stack fsG x)
 
 unfold
 let fs_oval_lambda
   (#g :typ_env)
   (#a :qType)
   (#b :qType)
-  (#wpBody : spec_env (extend a g) b)
-  (body :fs_oval (extend a g) b wpBody)
-  : fs_oval g (a ^-> b) (spec_env_lambda_tot body) by (
-  norm [delta_only [`%fs_val; `%op_Hat_Subtraction_Greater; `%get_Type]]; (** not sure why I have to do this **)
-  simpl ())
+  (#preBody : spec_env (extend a g))
+  (body :fs_oval (extend a g) b preBody)
+  : fs_oval g (a ^-> b) (spec_env_lambda_tot body)
   = fun fsG ->
       fun x -> body (stack fsG x)
 
 unfold
 val fs_oval_eq_string :
   #g : typ_env ->
-  #wpS1 : spec_env g qString ->
-  s1 : fs_oval g qString wpS1 ->
-  #wpS2 : spec_env g qString ->
-  s2 : fs_oval g qString wpS2 ->
-  fs_oval g qBool (spec_env_bind' wpS1 (fun s1' -> spec_env_bind' wpS2 (fun s2' -> spec_env_return (s1' = s2'))))
-let fs_oval_eq_string #_ #wpS1 s1 #wpS2 s2 fsG =
-  M.elim_pure_wp_monotonicity (wpS1 fsG);
-  M.elim_pure_wp_monotonicity (wpS2 fsG);
+  #preS1 : spec_env g ->
+  s1 : fs_oval g qString preS1 ->
+  #preS2 : spec_env g ->
+  s2 : fs_oval g qString preS2 ->
+  fs_oval g qBool (spec_env_app preS1 preS2)
+let fs_oval_eq_string #_ #preS1 s1 #preS2 s2 fsG =
   (s1 fsG) = (s2 fsG)
 
 val spec_env_if : #g :typ_env ->
-                #a :qType ->
-                wpC : spec_env g qBool ->
-                wpT : spec_env g a ->
-                wpE : spec_env g a ->
-                spec_env g a
-let spec_env_if #_ #a wpC wpT wpE =
-  (fun fsG ->
-    pure_bind_wp _ _ (wpC fsG) (fun r ->
-      pure_if_then_else _ r (wpT fsG) (wpE fsG)))
+                #preC : spec_env g ->
+                c : fs_oval g qBool preC ->
+                preT : spec_env g ->
+                preE : spec_env g ->
+                spec_env g
+let spec_env_if #_ #preC c preT preE =
+  (fun fsG -> preC fsG /\ (c fsG ==> preT fsG) /\ ((~(c fsG)) ==> preE fsG))
 
 unfold
 val fs_oval_if : #g :typ_env ->
                  #a  : qType ->
-                 #wpC : spec_env g qBool ->
-                 c   : fs_oval g qBool wpC ->
-                 #wpT : spec_env g a ->
-                 t   : fs_oval g a wpT ->
-                 #wpE : spec_env g a ->
-                 e   : fs_oval g a wpE ->
-                 fs_oval g a (spec_env_if wpC wpT wpE)
-let fs_oval_if #_ #_ #wpC c #wpT t #wpE e fsG =
-  M.elim_pure_wp_monotonicity (wpC fsG);
-  M.elim_pure_wp_monotonicity (wpT fsG);
-  M.elim_pure_wp_monotonicity (wpE fsG);
+                 #preC : spec_env g ->
+                 c   : fs_oval g qBool preC ->
+                 #preT : spec_env g ->
+                 t   : fs_oval g a preT ->
+                 #preE : spec_env g ->
+                 e   : fs_oval g a preE ->
+                 fs_oval g a (spec_env_if c preT preE)
+let fs_oval_if #_ #_ #preC c #preT t #preE e fsG =
   if c fsG then t fsG else e fsG
 
 unfold
 val fs_oval_pair : #g : typ_env ->
                    #a : qType ->
                    #b : qType ->
-                   #wpX : spec_env g a ->
-                   x : fs_oval g a wpX ->
-                   #wpY : spec_env g b ->
-                   y : fs_oval g b wpY ->
-                   fs_oval g (a ^* b) (spec_env_bind' wpX (fun x -> spec_env_bind' wpY (fun y -> spec_env_return (x, y))))
-let fs_oval_pair #_ #_ #_ #wpX x #wpY y fsG =
-  M.elim_pure_wp_monotonicity (wpX fsG);
-  M.elim_pure_wp_monotonicity (wpY fsG);
+                   #preX : spec_env g ->
+                   x : fs_oval g a preX ->
+                   #preY : spec_env g ->
+                   y : fs_oval g b preY ->
+                   fs_oval g (a ^* b) (spec_env_app preX preY)
+let fs_oval_pair #_ #_ #_ #preX x #preY y fsG =
   fs_val_pair (x fsG) (y fsG)
 
 val spec_env_case : #g :typ_env ->
                 #a :qType ->
                 #b  : qType ->
-                #c  : qType ->
-                wpCond : spec_env g (a ^+ b) ->
-                wpInlc : spec_env (extend a g) c ->
-                wpInrc : spec_env (extend b g) c ->
-                spec_env g c
-let spec_env_case wpCond wpInlc wpInrc =
-  (fun fsG ->
-    pure_bind_wp _ _ (wpCond fsG) (fun r ->
-      match r with
-      | Inl x -> wpInlc (stack fsG x)
-      | Inr x -> wpInrc (stack fsG x)))
+                #preCond : spec_env g ->
+                cond : fs_oval g (a ^+ b) preCond ->
+                preInlc : spec_env (extend a g) ->
+                preInrc : spec_env (extend b g) ->
+                spec_env g
+let spec_env_case #_ #_ #_ #preCond cond preInlc preInrc =
+  (fun fsG -> preCond fsG /\
+    (Inl? (cond fsG) ==> preInlc (stack fsG (Inl?.v (cond fsG)))) /\
+    (Inr? (cond fsG) ==> preInrc (stack fsG (Inr?.v (cond fsG)))))
 
 unfold
 val fs_oval_case : #g :typ_env ->
                   #a  : qType ->
                   #b  : qType ->
                   #c  : qType ->
-                  #wpCond : spec_env g (a ^+ b) ->
-                  cond: fs_oval g (a ^+ b) wpCond ->
-                  #wpInlc : spec_env (extend a g) c ->
-                  inlc: fs_oval (extend a g) c wpInlc ->
-                  #wpInrc : spec_env (extend b g) c ->
-                  inrc: fs_oval (extend b g) c wpInrc ->
-                  fs_oval g c (spec_env_case wpCond wpInlc wpInrc)
-let fs_oval_case #_ #_ #_ #_ #wpCond cond #wpInlc inlc #wpInrc inrc fsG =
-  M.elim_pure_wp_monotonicity (wpCond fsG);
+                  #preCond : spec_env g ->
+                  cond: fs_oval g (a ^+ b) preCond ->
+                  #preInlc : spec_env (extend a g) ->
+                  inlc: fs_oval (extend a g) c preInlc ->
+                  #preInrc : spec_env (extend b g) ->
+                  inrc: fs_oval (extend b g) c preInrc ->
+                  fs_oval g c (spec_env_case cond preInlc preInrc)
+let fs_oval_case #_ #_ #_ #_ #preCond cond #preInlc inlc #preInrc inrc fsG =
   match cond fsG with
   | Inl x ->
-    M.elim_pure_wp_monotonicity (wpInlc (stack fsG x));
     inlc (stack fsG x)
   | Inr x ->
-    M.elim_pure_wp_monotonicity (wpInrc (stack fsG x));
     inrc (stack fsG x)
 
 (** Open computations **)
@@ -350,11 +278,10 @@ unfold
 val fs_ocomp_return_oval :
         #g:typ_env ->
         #a:qType ->
-        #wpX:spec_env g a ->
-        x:fs_oval g a wpX ->
-        fs_ocomp g a wpX
-let fs_ocomp_return_oval #_ #a #wpX x fsG =
-  M.elim_pure_wp_monotonicity (wpX fsG);
+        #preX:spec_env g ->
+        x:fs_oval g a preX ->
+        fs_ocomp g a preX
+let fs_ocomp_return_oval #_ #a #preX x fsG =
   io_return (x fsG)
 
 val fs_ocomp_return_val :
@@ -365,31 +292,16 @@ val fs_ocomp_return_val :
 let fs_ocomp_return_val g a x =
   fs_ocomp_return_oval (fs_oval_return g x)
 
-val lem_spec_env_bind_as_requires_split :
-  #g:typ_env ->
-  #a:qType ->
-  #b:qType ->
-  wpM : spec_env g a ->
-  wpK : (spec_env (extend a g) b) ->
-  fsG : eval_env g ->
-  Lemma 
-    (requires (as_requires (spec_env_bind wpM wpK fsG))) 
-    (ensures (as_requires (wpM fsG) /\ (forall x. as_requires (wpK (stack fsG x)))))
-let lem_spec_env_bind_as_requires_split #g #a #b wpM wpK fsG =
-  M.elim_pure_wp_monotonicity_forall ()
-
 unfold
 val fs_ocomp_bind : #g:typ_env ->
                     #a:qType ->
                     #b:qType ->
-                    #wpM : spec_env g a ->
-                    m:fs_ocomp g a wpM ->
-                    #wpK : (spec_env (extend a g) b) ->
-                    k:fs_ocomp (extend a g) b wpK ->
-                    fs_ocomp g b (spec_env_bind wpM wpK)
-let fs_ocomp_bind #g #_ #b #wpM m #wpK k fsG 
-  : Pure (fs_comp b) (as_requires ((spec_env_bind wpM wpK) fsG)) (fun _ -> True) =
-  lem_spec_env_bind_as_requires_split wpM wpK fsG;
+                    #preM : spec_env g ->
+                    m:fs_ocomp g a preM ->
+                    #preK : (spec_env (extend a g)) ->
+                    k:fs_ocomp (extend a g) b preK ->
+                    fs_ocomp g b (spec_env_bind preM preK)
+let fs_ocomp_bind #g #_ #b #preM m #preK k fsG =
   fs_comp_bind (m fsG) (fun x ->
     k (stack fsG x))
 
@@ -398,21 +310,21 @@ unfold
 val fs_ocomp_bind' : #g:typ_env ->
                     #a:qType ->
                     #b:qType ->
-                    #wpM : spec_env g a ->
-                    m:fs_ocomp g a wpM ->
-                    #wpK : (fs_val a -> spec_env g b) ->
-                    k:(x:fs_val a -> fs_ocomp g b (wpK x)) ->
-                    fs_ocomp g b (spec_env_bind' wpM wpK)
+                    #preM : spec_env g ->
+                    m:fs_ocomp g a preM ->
+                    #preK : (fs_val a -> spec_env g) ->
+                    k:(x:fs_val a -> fs_ocomp g b (preK x)) ->
+                    fs_ocomp g b (spec_env_bind' preM preK)
 let fs_ocomp_bind' m k =
   fs_ocomp_bind m (fun fsG -> k (hd fsG) (tail fsG))
 
 val fs_ocomp_fmap : #g:typ_env ->
                     #a:qType ->
                     #b:qType ->
-                    #wpP : spec_env g a ->
-                    p : fs_ocomp g a wpP ->
+                    #preP : spec_env g ->
+                    p : fs_ocomp g a preP ->
                     f : (fs_val a -> fs_val b) ->
-                    fs_ocomp g b (spec_env_bind' wpP (fun x -> spec_env_return_comp (io_return (f x))))
+                    fs_ocomp g b (spec_env_bind' #g #a preP (fun x -> spec_env_return_comp #g #b (io_return (f x))))
 let fs_ocomp_fmap p f =
   fs_ocomp_bind' p (fun p' ->
     fs_ocomp_return_val _ _ (f p'))
@@ -422,9 +334,9 @@ unfold
 val fs_ocomp_call :
         #g:typ_env ->
         o:io_ops ->
-        #wpArgs : spec_env g (q_io_args o) ->
-        args:fs_ocomp g (q_io_args o) wpArgs ->
-        fs_ocomp g (q_io_res o) (spec_env_bind' wpArgs (fun a -> spec_env_return_comp (io_call o a)))
+        #preArgs : spec_env g ->
+        args:fs_ocomp g (q_io_args o) preArgs ->
+        fs_ocomp g (q_io_res o) (spec_env_bind' #g #(q_io_args o) preArgs (fun a -> spec_env_return_comp #g #(q_io_res o) (io_call o a)))
 let fs_ocomp_call o args =
   fs_ocomp_bind' args (fun args' ->
     fs_ocomp_return _ (io_call o args'))
@@ -433,9 +345,9 @@ unfold
 val fs_ocomp_call_oval :
         #g:typ_env ->
         o:io_ops ->
-        #wpArgs : spec_env g (q_io_args o) ->
-        args:fs_oval g (q_io_args o) wpArgs ->
-        fs_ocomp g (q_io_res o) (spec_env_bind' wpArgs (fun a -> spec_env_return_comp (io_call o a)))
+        #preArgs : spec_env g ->
+        args:fs_oval g (q_io_args o) preArgs ->
+        fs_ocomp g (q_io_res o) (spec_env_bind' #g #(q_io_args o) preArgs (fun a -> spec_env_return_comp #g #(q_io_res o) (io_call o a)))
 let fs_ocomp_call_oval o args =
   fs_ocomp_call o (fs_ocomp_return_oval args)
 
@@ -443,25 +355,19 @@ unfold
 val spec_env_lambda_tot_ocomp : #g :typ_env ->
                 #a :qType ->
                 #b :qType ->
-                #wpBody:spec_env (extend a g) b ->
-                body:fs_ocomp (extend a g) b wpBody ->
-                spec_env g (a ^->!@ b)
+                #preBody:spec_env (extend a g) ->
+                body:fs_ocomp (extend a g) b preBody ->
+                spec_env g
 
-let spec_env_lambda_tot_ocomp #g #a #b #wpBody body fsG : pure_wp (fs_val (a ^->!@ b)) by (
-  norm [delta_only [`%fs_val; `%op_Hat_Subtraction_Greater; `%get_Type]]
-)= (** Cezar: this looks exactly like what F* generates **)
-  mk_pure_wp (fun (p:pure_post (fs_val (a ^->!@ b))) ->
-    (forall (x:a._1). auto_squash (wpBody (stack fsG x) (fun _ -> True))) /\
-    (pure_bind_wp _ _
-      (pure_return (fs_val (a ^->!@ b)) (fun x -> body (stack fsG x))))
-      (pure_return (fs_val (a ^->!@ b))) p)
+let spec_env_lambda_tot_ocomp #g #a #b #preBody body fsG : pure_pre =
+  forall (x:fs_val a). preBody (stack fsG x)
 
 unfold
 val fs_oval_lambda_ocomp : #g :typ_env ->
                 #a :qType ->
                 #b :qType ->
-                #wpBody : spec_env (extend a g) b ->
-                body :fs_ocomp (extend a g) b wpBody ->
+                #preBody : spec_env (extend a g) ->
+                body :fs_ocomp (extend a g) b preBody ->
                 fs_oval g (a ^->!@ b) (spec_env_lambda_tot_ocomp body)
 let fs_oval_lambda_ocomp #_ #_ #_ #_ body fsG x = body (stack fsG x)
 
@@ -470,51 +376,48 @@ val fs_ocomp_app_oval_oval :
                 #g : typ_env ->
                 #a : qType ->
                 #b : qType ->
-                #wpF : spec_env g (a ^->!@ b) ->
-                f :fs_oval g (a ^->!@ b) wpF ->
-                #wpX : spec_env g a ->
-                x :fs_oval g a wpX ->
-                fs_ocomp g b (spec_env_bind' wpF (fun f' -> spec_env_bind' wpX (fun x' -> spec_env_return_comp (f' x'))))
-let fs_ocomp_app_oval_oval #_ #_ #_ #wpF f #wpX x fsG =
-  M.elim_pure_wp_monotonicity (wpF fsG);
-  M.elim_pure_wp_monotonicity (wpX fsG);
+                #preF : spec_env g ->
+                f :fs_oval g (a ^->!@ b) preF ->
+                #preX : spec_env g ->
+                x :fs_oval g a preX ->
+                fs_ocomp g b (spec_env_app preF preX)
+let fs_ocomp_app_oval_oval #_ #_ #_ #preF f #preX x fsG =
   (f fsG) (x fsG)
 
 unfold
 val fs_ocomp_if_val : #g :typ_env ->
                 #a  : qType ->
                 c   : fs_val qBool ->
-                #wpT : spec_env g a ->
-                t   : fs_ocomp g a wpT ->
-                #wpE : spec_env g a ->
-                e   : fs_ocomp g a wpE ->
-                fs_ocomp g a (fun fsG -> if c then wpT fsG else wpE fsG)
+                #preT : spec_env g ->
+                t   : fs_ocomp g a preT ->
+                #preE : spec_env g ->
+                e   : fs_ocomp g a preE ->
+                fs_ocomp g a (fun fsG -> if c then preT fsG else preE fsG)
 let fs_ocomp_if_val c t e fsG =
   if c then t fsG else e fsG
 
 unfold
 val fs_ocomp_if_oval : #g :typ_env ->
                 #a  : qType ->
-                #wpC : spec_env g qBool ->
-                c   : fs_oval g qBool wpC ->
-                #wpT : spec_env g a ->
-                t   : fs_ocomp g a wpT ->
-                #wpE : spec_env g a ->
-                e   : fs_ocomp g a wpE ->
-                fs_ocomp g a (spec_env_bind' wpC (fun c' -> if c' then wpT else wpE))
-let fs_ocomp_if_oval #_ #_ #wpC c t e fsG =
-  M.elim_pure_wp_monotonicity (wpC fsG);
-  fs_ocomp_if_val (c fsG) t e fsG
+                #preC : spec_env g ->
+                c   : fs_oval g qBool preC ->
+                #preT : spec_env g ->
+                t   : fs_ocomp g a preT ->
+                #preE : spec_env g ->
+                e   : fs_ocomp g a preE ->
+                fs_ocomp g a (spec_env_if c preT preE)
+let fs_ocomp_if_oval #_ #_ #preC c t e fsG =
+  if c fsG then t fsG else e fsG
 
 val fs_ocomp_if : #g :typ_env ->
                   #a : qType ->
-                  #wpC : spec_env g qBool ->
-                  c  : fs_ocomp g qBool wpC ->
-                  #wpT : spec_env g a ->
-                  t  : fs_ocomp g a wpT ->
-                  #wpE : spec_env g a ->
-                  e  : fs_ocomp g a wpE ->
-                  fs_ocomp g a (spec_env_bind' wpC (fun c' -> if c' then wpT else wpE))
+                  #preC : spec_env g ->
+                  c  : fs_ocomp g qBool preC ->
+                  #preT : spec_env g ->
+                  t  : fs_ocomp g a preT ->
+                  #preE : spec_env g ->
+                  e  : fs_ocomp g a preE ->
+                  fs_ocomp g a (spec_env_bind' #g #qBool preC (fun c' -> if c' then preT else preE))
 let fs_ocomp_if c t e =
   fs_ocomp_bind' c (fun c' -> fs_ocomp_if_val c' t e)
 
@@ -524,11 +427,11 @@ val fs_ocomp_case_val : #g :typ_env ->
                 #b : qType ->
                 #c : qType ->
                 cond : fs_val (a ^+ b) ->
-                #wpInlc : spec_env (extend a g) c ->
-                inlc : fs_ocomp (extend a g) c wpInlc ->
-                #wpInrc : spec_env (extend b g) c ->
-                inrc : fs_ocomp (extend b g) c wpInrc ->
-                fs_ocomp g c (fun fsG -> match cond with | Inl x -> wpInlc (stack fsG x) | Inr x -> wpInrc (stack fsG x))
+                #preInlc : spec_env (extend a g) ->
+                inlc : fs_ocomp (extend a g) c preInlc ->
+                #preInrc : spec_env (extend b g) ->
+                inrc : fs_ocomp (extend b g) c preInrc ->
+                fs_ocomp g c (fun fsG -> match cond with | Inl x -> preInlc (stack fsG x) | Inr x -> preInrc (stack fsG x))
 let fs_ocomp_case_val cond inlc inrc fsG =
   match cond with
   | Inl x -> inlc (stack fsG x)
@@ -539,52 +442,53 @@ val fs_ocomp_case_oval : #g :typ_env ->
                 #a  : qType ->
                 #b : qType ->
                 #c : qType ->
-                #wpCond : spec_env g (a ^+ b) ->
-                cond : fs_oval g (a ^+ b) wpCond ->
-                #wpInlc : spec_env (extend a g) c ->
-                inlc : fs_ocomp (extend a g) c wpInlc ->
-                #wpInrc : spec_env (extend b g) c ->
-                inrc : fs_ocomp (extend b g) c wpInrc ->
-                fs_ocomp g c (spec_env_case wpCond wpInlc wpInrc)
-let fs_ocomp_case_oval #_ #_ #_ #_ #wpCond cond inlc inrc fsG =
-  M.elim_pure_wp_monotonicity (wpCond fsG);
-  fs_ocomp_case_val (cond fsG) inlc inrc fsG
+                #preCond : spec_env g ->
+                cond : fs_oval g (a ^+ b) preCond ->
+                #preInlc : spec_env (extend a g) ->
+                inlc : fs_ocomp (extend a g) c preInlc ->
+                #preInrc : spec_env (extend b g) ->
+                inrc : fs_ocomp (extend b g) c preInrc ->
+                fs_ocomp g c (spec_env_case cond preInlc preInrc)
+let fs_ocomp_case_oval #_ #_ #_ #_ #preCond cond inlc inrc fsG =
+  match cond fsG with
+  | Inl x -> inlc (stack fsG x)
+  | Inr x -> inrc (stack fsG x)
 
 val fs_ocomp_case : #g :typ_env ->
                 #a  : qType ->
                 #b : qType ->
                 #c : qType ->
-                #wpCond : spec_env g (a ^+ b) ->
-                cond : fs_ocomp g (a ^+ b) wpCond ->
-                #wpInlc : spec_env (extend a g) c ->
-                inlc : fs_ocomp (extend a g) c wpInlc ->
-                #wpInrc : spec_env (extend b g) c ->
-                inrc : fs_ocomp (extend b g) c wpInrc ->
-                fs_ocomp g c (spec_env_bind' wpCond (fun cond' -> fun fsG -> match cond' with | Inl x -> wpInlc (stack fsG x) | Inr x -> wpInrc (stack fsG x)))
+                #preCond : spec_env g ->
+                cond : fs_ocomp g (a ^+ b) preCond ->
+                #preInlc : spec_env (extend a g) ->
+                inlc : fs_ocomp (extend a g) c preInlc ->
+                #preInrc : spec_env (extend b g) ->
+                inrc : fs_ocomp (extend b g) c preInrc ->
+                fs_ocomp g c (spec_env_bind' #g #(a ^+ b) preCond (fun cond' -> fun fsG -> match cond' with | Inl x -> preInlc (stack fsG x) | Inr x -> preInrc (stack fsG x)))
 let fs_ocomp_case cond inlc inrc =
   fs_ocomp_bind' cond (fun cond' ->
     fs_ocomp_case_val cond' inlc inrc)
 
-let fs_ocomp_var (g:typ_env) (x:var{Some? (g x)}) : fs_ocomp g (Some?.v (g x)) (spec_env_bind' (spec_env_index x) (fun v -> spec_env_return_comp (io_return v))) =
+let fs_ocomp_var (g:typ_env) (x:var{Some? (g x)}) : fs_ocomp g (Some?.v (g x)) (spec_env_bind' #g #(Some?.v (g x)) (spec_env_index x) (fun v -> spec_env_return_comp #g #(Some?.v (g x)) (io_return v))) =
   fs_ocomp_return_oval (fs_oval_var g x)
 
 val fs_ocomp_lambda : #g :typ_env ->
                 #a :qType ->
                 #b :qType ->
-                #wpBody : spec_env (extend a g) b ->
-                body :fs_ocomp (extend a g) b wpBody ->
-                fs_ocomp g (a ^->!@ b) (spec_env_bind' (spec_env_lambda_tot_ocomp body) (fun x -> spec_env_return_comp (io_return x)))
+                #preBody : spec_env (extend a g) ->
+                body :fs_ocomp (extend a g) b preBody ->
+                fs_ocomp g (a ^->!@ b) (spec_env_bind' #g #(a ^->!@ b) (spec_env_lambda_tot_ocomp body) (fun x -> spec_env_return_comp #g #(a ^->!@ b) (io_return x)))
 let fs_ocomp_lambda body =
   fs_ocomp_return_oval (fs_oval_lambda_ocomp body)
 
 val fs_ocomp_app : #g:typ_env ->
                     #a:qType ->
                     #b:qType ->
-                    #wpF : spec_env g (a ^->!@ b) ->
-                    f:fs_ocomp g (a ^->!@ b) wpF ->
-                    #wpX : spec_env g a ->
-                    x:fs_ocomp g a wpX ->
-                    fs_ocomp g b (spec_env_bind' wpF (fun f' -> spec_env_bind' wpX (fun x' -> spec_env_return_comp (f' x'))))
+                    #preF : spec_env g ->
+                    f:fs_ocomp g (a ^->!@ b) preF ->
+                    #preX : spec_env g ->
+                    x:fs_ocomp g a preX ->
+                    fs_ocomp g b (spec_env_bind' #g #(a ^->!@ b) preF (fun f' -> spec_env_bind' #g #a preX (fun x' -> spec_env_return_comp #g #b (f' x'))))
 let fs_ocomp_app f x =
   fs_ocomp_bind' f (fun f' ->
     fs_ocomp_bind' x (fun x' ->
@@ -593,22 +497,22 @@ let fs_ocomp_app f x =
 val fs_ocomp_pair : #g : typ_env ->
                    #a : qType ->
                    #b : qType ->
-                   #wpX : spec_env g a ->
-                   x : fs_ocomp g a wpX ->
-                   #wpY : spec_env g b ->
-                   y : fs_ocomp g b wpY ->
-                   fs_ocomp g (a ^* b) (spec_env_bind' wpX (fun x' -> spec_env_bind' wpY (fun y' -> spec_env_return_comp (io_return (fs_val_pair x' y')))))
+                   #preX : spec_env g ->
+                   x : fs_ocomp g a preX ->
+                   #preY : spec_env g ->
+                   y : fs_ocomp g b preY ->
+                   fs_ocomp g (a ^* b) (spec_env_bind' #g #a preX (fun x' -> spec_env_bind' #g #b preY (fun y' -> spec_env_return_comp #g #(a ^* b) (io_return (fs_val_pair x' y')))))
 let fs_ocomp_pair x y =
   fs_ocomp_bind' x (fun x' ->
     fs_ocomp_bind' y (fun y' ->
       fs_ocomp_return_val _ _ (fs_val_pair x' y')))
 
 val fs_ocomp_string_eq : #g : typ_env ->
-                         #wpX : spec_env g qString ->
-                         x : fs_ocomp g qString wpX ->
-                         #wpY : spec_env g qString ->
-                         y : fs_ocomp g qString wpY ->
-                         fs_ocomp g qBool (spec_env_bind' wpX (fun x' -> spec_env_bind' wpY (fun y' -> spec_env_return_comp (io_return (x' = y')))))
+                         #preX : spec_env g ->
+                         x : fs_ocomp g qString preX ->
+                         #preY : spec_env g ->
+                         y : fs_ocomp g qString preY ->
+                         fs_ocomp g qBool (spec_env_bind' #g #qString preX (fun x' -> spec_env_bind' #g #qString preY (fun y' -> spec_env_return_comp #g #qBool (io_return (x' = y')))))
 let fs_ocomp_string_eq x y =
   fs_ocomp_bind' x (fun x' ->
     fs_ocomp_bind' y (fun y' ->
